Moved some proofs from AbstractMultiPaxosR3 to R3_Refines_R1 and removed a duplicate definition from DistributedSafeAt.

Isabelle2/DistributedSafeAt.thy
@@ -3,8 +3,6 @@ imports BallotArrays BallotArrayProperties "~~/src/HOL/Library/Monad_Syntax" Uti
 begin
 
 subsection {* Computing safe values in a distributed implementation *}
-
-definition option_as_set where "option_as_set x \<equiv> case x of None \<Rightarrow> {} | Some y \<Rightarrow> {y}"
   
 locale distributed_safe_at = ballot_array
 begin
