Isabelle2/R3_Refines_R1.thy
@@ -4,6 +4,60 @@ theory R3_Refines_R1
 imports AbstractMultiPaxosR3 AbstractMultiPaxosR1 Simulations Hist_Supplemental IOA_Automation
 begin
 
+locale receive_1b_lemmas = receive_1b votes as log for votes as log +
+  assumes votes_default:"\<And> a . finfun_default (votes $ a) = None"
+    and log_default:"finfun_default log = amp_r3.inst_status.Free" and fin:"finite as"
+begin
+
+lemma per_inst_lemma:
+  "\<And> ff . ff \<in> per_inst \<Longrightarrow> finfun_default ff = None"
+  using receive_1b_lemmas_axioms receive_1b_lemmas_def
+  using per_inst_def by (metis (mono_tags, lifting) imageE)
+
+lemma votes_per_inst_lemma:
+  fixes s assumes "finite s" and "\<And> ff . ff \<in> s \<Longrightarrow> finfun_default ff = None"
+  shows "finfun_default (votes_per_inst s) = {}"
+proof (simp add:votes_per_inst_def)
+  show "finfun_default (Finite_Set.fold combine (K$ {}) s) = {}" using assms
+  proof (induct s)
+    case empty
+    then show ?case by (simp add:combine_def finfun_default_const)
+  next
+    case (insert x F)
+    have 1:"Finite_Set.fold combine (K$ {}) (insert x F)
+      = combine x (Finite_Set.fold combine (K$ {}) F)" using insert_idem
+      by (metis eq_fold insert.hyps(1))
+    have "finfun_default (Finite_Set.fold combine (K$ {}) F) = {}"
+      by (simp add: insert.hyps(3) insert.prems)
+    moreover have "finfun_default x = None"
+      by (simp add: insert.prems) 
+    ultimately have "finfun_default ($ x, Finite_Set.fold combine (K$ {}) F $) = (None, {})"
+      by (simp add: diag_default)
+    hence "finfun_default ( (\<lambda>(vo, vs). option_as_set vo \<union> vs) \<circ>$
+                 ($x, Finite_Set.fold combine (K$ {}) F$)) = {}"
+      by (simp add:comp_default option_as_set_def)
+    thus ?case apply (simp add:1) by (auto simp add:combine_def) 
+  qed
+qed
+
+lemma max_per_inst_default:
+  "finfun_default (max_per_inst) = {}"
+proof -
+  have "finfun_default (votes_per_inst per_inst) = {}"
+  proof -
+    have "finite per_inst" using fin by (simp add:per_inst_def)
+    thus ?thesis by (simp add:per_inst_lemma votes_per_inst_lemma)
+  qed
+  thus ?thesis by (simp add:max_per_inst_def max_by_key_def comp_default)
+qed
+
+lemma new_log_lemma:
+  "finfun_default new_log = amp_r3.inst_status.Free" using log_default
+  apply (auto simp add:new_log_def max_per_inst_default comp_default diag_default)
+  by (simp add: amp_r3.inst_status.simps(11))
+  
+end
+
 section {* A first attempt. *}
 
 locale ref_proof_1 = quorums quorums + amp_r3 leader next_bal as quorums 
@@ -318,7 +372,7 @@ lemma inv2:"invariant ampr3_ioa inv2"
   apply (instantiate_invs)
   apply (rm_reachable)
   apply trans_cases
-         apply (simp_all add:inv2_def inv1_def action_defs split!:if_splits) 
+         apply (simp_all add:inv2_def inv1_def action_defs split!:if_splits)
   oops
   
 definition inv3 where 
